

## More on Causality, Invertibility, Introduction to Forecasting and Estimation

### Exercise 1 (Consequences of Causality)

Recall the AR(2) process from the last problem set.

$$y_t = 0.7y_{t-1} - 0.1y_{t-2} + \varepsilon_t, \quad \{\varepsilon_t\} \sim \text{GWN}(0, \sigma^2), \quad t \in \mathbb{Z}. \quad (1)$$

Since this process is weakly stationary and causal, derive the MA( $\infty$ ) representation of (1).

**Hint:** Derive the recursive relationship

$$\phi_j = \phi_{j-1}\alpha_1 + \phi_{j-2}\alpha_2,$$

where the  $\phi_i$ 's correspond to the coefficients of the MA( $\infty$ )-polynomial

$$\phi(L) = \phi_0 + \phi_1 L + \phi_2 L^2 + \dots$$

such that  $x_t = \phi(L)\varepsilon_t$ . The recursive relation stated above can be transformed into a homogeneous 2<sup>nd</sup> order difference equation

$$\phi_j - \phi_{j-1}\alpha_1 - \phi_{j-2}\alpha_2 = 0.$$

The solution (see Shumway & Stoffer 2011 section 3.3) can be written as

$$\phi_j = c_1 k_1^j + c_2 k_2^j,$$

where  $k_1, k_2$  are the reciprocal values of the characteristic roots  $\lambda_1, \lambda_2$  (with  $\lambda_1 \neq \lambda_2$ ) of the AR polynomial  $a(\lambda) = 1 - \alpha_1\lambda - \alpha_2\lambda^2 = 0$ .

For causal and weakly stationary ARMA processes it holds

$$\begin{aligned} a(L)x_t &= b(L)\varepsilon_t \\ \Rightarrow x_t &= \frac{b(L)}{a(L)}\varepsilon_t = \phi(L)\varepsilon_t. \end{aligned}$$

We write the polynomial  $\phi(L)$  as a function of  $\lambda \in \mathbb{C}$ ,

$$\begin{aligned} \phi(\lambda) &= \sum_{j=0}^{\infty} \phi_j \lambda^j \left( = \frac{b(\lambda)}{a(\lambda)} \right) \\ \Leftrightarrow \phi(\lambda)a(\lambda) &= b(\lambda). \end{aligned}$$

For the given parameter combination, i.e., the stated AR(2)-process we get

$$\begin{aligned}
 & (\phi_0 + \phi_1\lambda + \phi_2\lambda^2 + \dots)(1 - \alpha_1\lambda - \alpha_2\lambda^2) = 1 \\
 \Leftrightarrow & \phi_0 - \phi_0\alpha_1\lambda - \phi_0\alpha_2\lambda^2 \\
 & + \phi_1\lambda - \phi_1\alpha_1\lambda^2 - \phi_1\alpha_2\lambda^3 \\
 & + \phi_2\lambda^2 - \phi_2\alpha_1\lambda^3 - \dots \\
 & + \dots = 1.
 \end{aligned}$$

Applying the method of matching coefficients gives

$$\begin{aligned}
 \phi_0 &= 1 \\
 \phi_1 - \phi_0\alpha_1 &= 0 \Rightarrow \phi_1 = \alpha_1 \\
 \phi_2 - \phi_1\alpha_1 - \phi_0\alpha_2 &= 0 \Rightarrow \phi_2 = \phi_1\alpha_1 + \phi_0\alpha_2 = \alpha_1^2 + \alpha_2 \\
 &\vdots
 \end{aligned}$$

Altogether we obtain the recursive relationship

$$\phi_j = \phi_{j-1}\alpha_1 + \phi_{j-2}\alpha_2.$$

The solution is given by (hint)

$$\phi_j = c_1 k_1^j + c_2 k_2^j,$$

with

$$k_1 = \frac{1}{2} = 0.5 \text{ and } k_2 = \frac{1}{5} = 0.2.$$

Using the initial conditions gives

$$\begin{aligned}
 1 &= \phi_0 = c_1 0.5^0 + c_2 0.2^0 \\
 \alpha_1 = 0.7 &= \phi_1 = c_1 0.5^1 + c_2 0.2^1;
 \end{aligned}$$

Solving the system of equations implies

$$\begin{aligned}
 -0.4 &= 0.6c_2 \\
 c_2 &= -\frac{2}{3} \\
 c_1 &= \frac{5}{3}.
 \end{aligned}$$

**Exercise 2** (Uniqueness and invertibility of MA processes)

**Recall:** A linear process is called **invertible**, if and only if there exists a polynomial

$$\pi(L) = \pi_0 + \pi_1 L + \pi_2 L^2 + \dots$$

such that

$$\varepsilon_t = \pi(L)x_t.$$

(a) Show that the two MA(1) processes

$$\begin{aligned} x_t &= \varepsilon_t + \beta_1 \varepsilon_{t-1} & \{\varepsilon_t\} &\sim \text{WN}(0, \sigma^2) \\ y_t &= \epsilon_t + \frac{1}{\beta_1} \epsilon_{t-1} & \{\epsilon_t\} &\sim \text{WN}(0, \sigma^2 \beta_1^2) \end{aligned}$$

where  $0 < |\beta_1| < 1$ , have the same autocovariance functions.

In Problem Set 2 exercise 1, we derived the autocovariance function of the first MA(1) process.

$$\gamma_x(h) = \begin{cases} \sigma^2(1 + \beta_1^2), & h = 0, \\ \beta_1 \sigma^2, & |h| = 1, \\ 0, & |h| > 1. \end{cases}$$

For  $y_t$  it then follows:

$$\gamma_y(h) = \begin{cases} \sigma^2 \beta_1^2 (1 + \frac{1}{\beta_1^2}) = \sigma^2(1 + \beta_1^2), & h = 0, \\ \frac{1}{\beta_1} \sigma^2 \beta_1^2 = \beta_1 \sigma^2, & |h| = 1, \\ 0, & |h| > 1. \end{cases}$$

Thus the equality follows.

- (b) MA processes that can be represented by an infinite AR representation are called invertible. Write down the AR representations for both processes. Which one is invertible?

$$x_t = \varepsilon_t + \beta_1 \varepsilon_{t-1} \iff \varepsilon_t = x_t - \beta_1 \varepsilon_{t-1}$$

Through substitution of all  $\varepsilon$  we get:

$$\begin{aligned} \varepsilon_t &= x_t - \beta_1 \varepsilon_{t-1} \\ &= -\beta(-\beta \varepsilon_{t-2} + x_{t-1}) + x_t \\ &= \dots \\ &= \sum_{i=0}^{\infty} (-\beta_1)^i x_{t-j} \end{aligned}$$

For  $y_t$  the procedure is the same

$$\begin{aligned} \epsilon_t &= y_t - \frac{1}{\beta_1} \epsilon_{t-1} \\ &= -\frac{1}{\beta_1} \left( -\frac{1}{\beta_1} \epsilon_{t-2} + y_{t-1} \right) + y_t \\ &= \dots \\ &= \sum_{i=0}^{\infty} \left( -\frac{1}{\beta_1} \right)^i y_{t-j} \end{aligned}$$

Since  $|\beta_1| < 1$ , it follows  $|\frac{1}{\beta_1}| > 1$ , therefore  $x_t$  is invertible and  $y_t$  is not because the sum is not well-defined.

**Exercise 3** (Forecasting stationary processes)

Suppose we would like to predict a single stationary series  $\{x_t\}_t$  with zero mean and autocovariance function  $\gamma(h)$  at some time in the future, say,  $t + \ell$ , for  $\ell > 0$ .

- (a) If we predict using  $x_t$  and some scale multiplier  $A$  only, show that the mean-square prediction error

$$MSE(A) = E[(x_{t+\ell} - Ax_t)^2], \quad (2)$$

is being minimized by

$$A = \rho(\ell). \quad (3)$$

Rewrite the MSE:

$$\begin{aligned} MSE(A) &= E(x_{t+\ell}^2 - 2Ax_tx_{t+\ell} + A^2x_t^2) \\ &= E(x_{t+\ell}^2) - 2AE(x_tx_{t+\ell}) + A^2E(x_t^2) \\ &= \gamma(0) - 2A\gamma(\ell) + A^2\gamma(0) \\ &= (1 + A^2)\gamma(0) - 2A\gamma(\ell). \end{aligned}$$

Partial derivative:

$$\frac{\partial MSE(A)}{\partial A} = 2A\gamma(0) - 2\gamma(\ell).$$

Solve

$$2A\gamma(0) - 2\gamma(\ell) \stackrel{!}{=} 0,$$

which gives

$$A = \frac{\gamma(\ell)}{\gamma(0)} = \rho(\ell).$$

This solution yields a minimum because

$$\frac{\partial^2 MSE(A)}{\partial A^2} = 2\gamma(0) = 2E(x_t^2) > 0.$$

- (b) Show that in this case the minimum mean-square prediction error is given by

$$MSE(A) = \gamma(0)[1 - \rho^2(\ell)]. \quad (4)$$

The minimum is given by

$$\begin{aligned} MSE(A_{min}) &= (1 + \rho(\ell)^2)\gamma(0) - 2\rho(\ell)\gamma(\ell) \\ &= (1 + \rho(\ell)^2)\gamma(0) - 2\rho(\ell)\rho(\ell)\gamma(0) \\ &= \gamma(0)[1 - \rho(\ell)^2] \end{aligned}$$

**Exercise 4** (Yule-Walker equations and a first look at estimation)

Consider the AR(2) process

$$y_t = \alpha_1 y_{t-1} + \alpha_2 y_{t-2} + \varepsilon_t, \quad \varepsilon_t \stackrel{iid}{\sim} GWN(0, \sigma^2), \quad t \in \mathbb{Z} \quad (5)$$

where *GWN* means *Gaussian white noise*. Furthermore, assume that this process is causal.

- (a) Derive the Yule-Walker equations of the process, and determine its ACF for the first two lags,  $\rho(1)$  and  $\rho(2)$ .

Multiply the base equation with  $y_{t-h}$  and take the expectation yields

$$E(y_t y_{t-h}) = \alpha_1 E(y_{t-1} y_{t-h}) + \alpha_2 E(y_{t-2} y_{t-h}) + E(\varepsilon_t y_{t-h}). \quad (6)$$

Note, that it holds

$$E(\varepsilon_t y_{t-h}) = \begin{cases} \sigma^2 & , h = 0, \\ 0 & , \text{otherwise.} \end{cases}$$

Altogether we get

$$\gamma(0) = \alpha_1 \gamma(1) + \alpha_2 \gamma(2) + \sigma^2 \quad \text{for } h = 0 \quad (7)$$

$$\gamma(h) = \alpha_1 \gamma(h-1) + \alpha_2 \gamma(h-2) \quad \text{for } h = \pm 1, \pm 2, \dots, \quad (8)$$

which are the so-called **Yule-Walker equations**. For  $h = 1, 2$  the ACF is given by

$$\begin{aligned} \rho(1) &= \frac{\gamma(1)}{\gamma(0)} = \frac{\alpha_1 \gamma(0) + \alpha_2 \gamma(1)}{\gamma(0)} \\ &= \alpha_1 + \alpha_2 \rho(1) \\ \Rightarrow \rho(1) &= \frac{\alpha_1}{1 - \alpha_2}; \\ \rho(2) &= \frac{\gamma(2)}{\gamma(0)} = \frac{\alpha_1 \gamma(1) + \alpha_2 \gamma(0)}{\gamma(0)} \\ &= \alpha_1 \rho(1) + \alpha_2 \\ &= \frac{\alpha_1^2}{1 - \alpha_2} + \alpha_2 \\ \Rightarrow \rho(2) &= \frac{\alpha_1^2 + \alpha_2 - \alpha_2^2}{1 - \alpha_2}. \end{aligned}$$

- (b) Find the variance of  $\{y_t\}_t$ .

With (??) it follows

$$\begin{aligned} \sigma^2 &= \gamma(0) - \alpha_1 \gamma(1) - \alpha_2 \gamma(2) \\ &= \gamma(0) - \alpha_1 \rho(1) \gamma(0) - \alpha_2 \rho(2) \gamma(0) \\ &= \gamma(0) (1 - \alpha_1 \rho(1) - \alpha_2 \rho(2)) \end{aligned}$$

implying

$$\begin{aligned}\gamma(0) &= \frac{\sigma^2}{1 - \frac{\alpha_1^2}{1-\alpha_2} - \alpha_2 \frac{\alpha_1^2 + \alpha_2 - \alpha_2^2}{1-\alpha_2}} \\ &= \frac{(1 - \alpha_2)\sigma^2}{1 - \alpha_2 - \alpha_1^2 - \alpha_2\alpha_1^2 - \alpha_2^2 + \alpha_2^3}.\end{aligned}$$